Destroy our memory model to give up on external function calls.
This is useful since we can now talk about enriching traces with the
value of memory. That is, we can write a function:

mem_effect: Mem -> Trace X -> Trace (Memory * X)

where the leaf nodes are enriched with the state of memory at that
point. The downside is that our memory model gives up when there is an
external function call and returns am "Err"

The less destructive path would have been to have a coinductive
predicate (in Prop) `TraceDoesNotContainExternalFunctionCall`
that the trace does not contain external function
calls. So we would write a function:

mem_effect: Mem -> (x: Trace X)
                -> TraceDoesNotContainExternalFunctionCall x
                -> Trace (Memory * X)

However, Tobias had a convincing argument that this extra proof
engineering is not worth the effort, which I agree with. We can amend
this later if need be.

This is nice, because we can now talk about memory effects on infinite
traces without having to provide an explicit witness (in Type) about the
finiteness of the trace.

src/coq/Memory.v
@@ -304,7 +304,7 @@ CoFixpoint memD {X} (m:memory) (d:Trace X) : Trace X :=
   | Trace.Vis _ io k =>
     match mem_step io m with
     | inr (m', v) => Trace.Tau (memD m' (k v))
-    | inl e => Trace.Vis io k
+    | inl e => Trace.Err "uninterpretiable IO call" (* Trace.Vis io k *)
     end
   | Trace.Ret x => d
   | Trace.Err x => d
@@ -347,13 +347,13 @@ CoFixpoint mem_effect_1 {X} (m: memory) (tx: Trace X):
   Trace (memory * X) :=
   (* (Trace memory) * (Trace X) := *)
   match tx with
-  | Trace.Ret x => (Trace.Ret (m,  x))
+  | Trace.Ret x => (Trace.Ret ( m,  x))
   | Trace.Err e => Trace.Err e
   | Trace.Tau x' =>  Trace.Tau (mem_effect_1 m x')
   | Trace.Vis Y io k => 
     match mem_step io m with
     | inr (m', v) => Trace.Tau (mem_effect_1 m' (k v))
-    | inl e => Trace.Vis io (fun y => Trace.mapM (fun x => (m, x)) (k y))
+    | inl e => Trace.Err "uninterpretiable IO call "
     end
   end.
   
@@ -386,7 +386,7 @@ Fixpoint mem_effect_fin {X} (m: memory) (d: Trace X) (FIN: Trace.TraceFinite d)
                                 (* Is this correct..?*)
                                 let (m'', t) := mem_effect_fin m' (FINK v)
                                 in  (m'', Trace.Tau t)
-                              | inl e => (m, (Trace.Vis io k))
+                              | inl e => (m, Trace.Err "uninterpretiable IO call")
                               end
   end.
 
@@ -536,7 +536,7 @@ Lemma force_memD_vis:
     (mem: memory),
     memD mem  (Trace.Vis e k) ≡
     match mem_step e mem with
-    | inl _ => Trace.Vis e k
+    | inl _ => Trace.Err "uninterpretiable IO call"
     | inr (m', v) => Trace.Tau (memD m' (k v))
     end.
 Proof.
@@ -703,6 +703,10 @@ Proof.
     simpl.
     destruct (mem_step e m) eqn:MEMSTEP.
     + euttnorm.
+      forcememd.
+      rewrite MEMSTEP.
+      forcememd.
+      
     + euttnorm.
       destruct p eqn:P.
       subst.
@@ -747,7 +751,9 @@ Theorem memD_commutes_with_bind_mem_effect_1: forall {X Y: Type}
                                  (m: memory),
     memD m (bindM trx f) ≡
             bindM (mem_effect_1 m trx)
-            (fun out =>  memD (fst out) (bindM (Ret (snd out)) f)).
+            (fun out =>  match out with
+                      | (m', x) => memD m' (bindM (Ret x) f)
+                      end).
 Proof.
   intros until Y.
   cofix CIH.
@@ -764,22 +770,11 @@ Proof.
     destruct (mem_step e m) eqn:MEMSTEP.
     + euttnorm.
       constructor.
-      intros.
-      rewrite (@Trace.matchM) with (i := mapM _ _).
-      admit.
-
-      (* 
-      destruct (k y).
-      *  simpl.
-         rewrite (@Trace.matchM) with (i := bindM _ _); simpl.
-       *)
-
-      
     + destruct p.
-      rewrite (@Trace.matchM) with (i := bindM (Tau _) _).
+      rewrite (@Trace.matchM) with (i := bindM _ _); simpl.
+      constructor.
       Guarded.
       simpl.
-      constructor.
       apply CIH with (m := m0) (trx := (k y)) (f :=f).
       Guarded.
 
@@ -798,68 +793,8 @@ Proof.
     euttnorm.
     forcememd.
     Guarded.
-Abort.
-
-(**
-memD m (trx >>= f) ≡
-    (mem_effect m trx) >>= \((m', trx') -> memD m' (trx' >>= f))
-**)
-Theorem memD_commutes_with_bind_mem_effect_2: forall {X Y: Type}
-                                 (trx: Trace X)
-                                 (f: X -> Trace Y)
-                                 (m: memory),
-    memD m (bindM trx f) ≡
-            bindM (mem_effect_2 m trx)
-            (fun out =>  memD (fst out) (bindM (snd out) f)).
-Proof.
-  intros until f.
-  cofix CIH.
-  intros.
-  destruct trx.
-  - (* ret *)
-    euttnorm.
-    rewrite (@Trace.matchM) with (i := mem_effect_2 _ _); simpl; repeat progress euttnorm.
-  - (* vis *)
-    euttnorm.
-    rewrite (@Trace.matchM) with (i := mem_effect_2 _ _); simpl; repeat progress euttnorm.
-    forcememd.
-    destruct (mem_step e m) eqn:STEP.
-    + euttnorm.
-      admit.
-    + destruct p eqn:P.
-      euttnorm.
-Abort.
-
-
-Lemma bind_ret_is_identity: forall {X: Type} (trx: Trace X),
-    bindM trx (Ret (Event:=IO) (X:=X)) ≡ trx.
-Proof.
-  intros X.
-  cofix CIH.
-
-  intros.
-  rewrite @Trace.matchM with (i := bindM _ _).
-
-  destruct trx; simpl.
-
-  - euttnorm.
-    Guarded.
-
-  - (* Vis *)
-    constructor.
-    intros. apply CIH.
-    Guarded.
-
-
-  - (* Tau*)
-    constructor.
-    apply CIH.
-    Guarded.
-
-  - euttnorm.
-    Guarded.
 Qed.
-    
+
 
 Theorem rewrite_memD_as_memEffect_fin: forall {X: Type}
                              (trx: Trace X)
